[SI] add simple specs. minor fixes in specs. added api as class.

aneris/examples/snapshot_isolation/specs/specs_hist.v
@@ -7,80 +7,81 @@ From aneris.aneris_lang.lib.serialization
      Require Import serialization_proof.
 From aneris.aneris_lang.program_logic Require Import lightweight_atomic.
 From aneris.examples.snapshot_isolation
-     Require Import snapshot_isolation_code.
+     Require Import snapshot_isolation_code_api.
 From aneris.examples.snapshot_isolation.specs
      Require Import user_params resources_hist.
 
 
 (** Specifications for read and write operations.  *)
 Section Specification.
-  Context `{!anerisG Mdl Σ, !User_params, !SI_resources Mdl Σ}.
+  Context `{!anerisG Mdl Σ, !User_params, !KVS_snapshot_isolation_api, !SI_resources Mdl Σ}.
 
   Definition write_spec : Prop :=
-    ∀ (rpc : val) (sa : socket_address)
+    ∀ (cstate : val) (sa : socket_address)
       (h : THst) (m : gmap Key val) E
       (k : Key) (v : SerializableVal),
     ⌜k ∈ KVS_keys⌝ -∗
-    {{{ TState rpc h m }}}
-      write rpc #k v @[ip_of_address sa] E
-    {{{ RET #(); TState rpc h (<[k:=v.(SV_val)]> m) }}}.
+    {{{ TState cstate h m }}}
+      SI_write cstate #k v @[ip_of_address sa] E
+    {{{ RET #(); TState cstate h (<[k:=v.(SV_val)]> m) }}}.
 
   Definition read_spec : Prop :=
-    ∀ (rpc : val) (sa : socket_address)
+    ∀ (cstate : val) (sa : socket_address)
     (h : THst) (m : gmap Key val) E
      (k : Key), ⌜k ∈ KVS_keys⌝ -∗
-    {{{ TState rpc h m }}}
-      read rpc #k @[ip_of_address sa] E
-    {{{ (vo : val), RET vo; TState rpc h m ∗
+    {{{ TState cstate h m }}}
+      SI_read cstate #k @[ip_of_address sa] E
+    {{{ (vo : val), RET vo; TState cstate h m ∗
         ⌜k ∉ dom m ∧ vo = $(get_current_state h !! k) ∨
          ∃ v, Some v = (m !! k) ∧ vo = $(Some v)⌝ }}}.
 
   Definition start_spec : Prop :=
-    ∀ (rpc : val) (sa : socket_address) (E : coPset),
+    ∀ (cstate : val) (sa : socket_address) (E : coPset),
     ⌜↑KVS_InvName ⊆ E⌝ -∗
     <<< ∀∀ (hl hg: THst),
-        LHist rpc sa hl ∗ GHist hg ∗ CanStart sa rpc >>>
-      start rpc #() @[ip_of_address sa] E
+        LHist cstate sa hl ∗ GHist hg ∗ CanStart sa cstate >>>
+      SI_start cstate @[ip_of_address sa] E
     <<<▷ RET #();
-        LHist rpc sa hl ∗ GHist hg ∗ TState rpc hg ∅ >>>.
+        LHist cstate sa hl ∗ GHist hg ∗ TState cstate hg ∅ >>>.
 
   Definition commit_spec : Prop :=
-   ∀ (rpc : val) (sa : socket_address) (E : coPset),
+   ∀ (cstate : val) (sa : socket_address)
+     (P : THst → iProp Σ)
+     (Q : THst → gmap Key val → iProp Σ)
+    (E : coPset),
     ⌜↑KVS_InvName ⊆ E⌝ -∗
     <<< ∀∀ (hl hs hg: THst) (m : gmap Key val),
-    LHist rpc sa hl ∗ GHist hg ∗ TState rpc hs m >>>
-      commit rpc #() @[ip_of_address sa] E
+    LHist cstate sa hl ∗ GHist hg ∗ TState cstate hs m ∗ P hs >>>
+      SI_commit cstate @[ip_of_address sa] E
     <<<▷∃∃ b, RET #b;
-          CanStart sa rpc ∗
+          CanStart sa cstate ∗
           (⌜b = true⌝ ∗ ⌜can_commit hs m hg⌝ ∗
-            GHist ((sa, m) :: hg) ∗ LHist rpc sa ((sa, m) :: hl)) ∨
-          (⌜b = false⌝ ∗ GHist hg ∗ LHist rpc sa hl) >>>.
+            GHist ((sa, m) :: hg) ∗ LHist cstate sa ((sa, m) :: hl) ∗ Q hs m) ∨
+          (⌜b = false⌝ ∗ ⌜¬ can_commit hs m hg⌝ ∗
+            GHist hg ∗ LHist cstate sa hl) >>>.
 
 (** TODO: Read only transaction *)
 
-(** Fixme *)
-(* I think that this spec is wrong! Because h in pre and post of atomic triple
-   should not be the same. *)
 Definition run_spec : Prop :=
-    ∀ (rpc : val) (tbody : val)
+    ∀ (cstate : val) (tbody : val)
       (sa : socket_address) (E : coPset)
       (m : gmap Key val) (h: THst) (hl : THst)
       (P : THst → iProp Σ)
       (Q : THst → gmap Key val → iProp Σ),
     ⌜↑KVS_InvName ⊆ E⌝
     -∗
-    {{{ TState rpc h ∅ ∗ P h }}}
-      tbody rpc #() @[ip_of_address sa] E
-    {{{ RET #(); TState rpc h m ∗ Q h m }}}
+    {{{ TState cstate h ∅ ∗ P h }}}
+      tbody cstate #() @[ip_of_address sa] E
+    {{{ RET #(); TState cstate h m ∗ Q h m }}}
     →
-    <<< ∀∀ (x : unit), CanStart sa rpc ∗ GHist h ∗ LHist rpc sa hl ∗ P h >>>
-           run rpc tbody #() @[ip_of_address sa] E
+    <<< ∀∀ (x : unit), CanStart sa cstate ∗ GHist h ∗ LHist cstate sa hl ∗ P h >>>
+           SI_run cstate tbody @[ip_of_address sa] E
     <<<▷∃∃ b h',  RET #b;
         ⌜h ≤ₚ h'⌝ ∗
-        CanStart sa rpc ∗
+        CanStart sa cstate ∗
         (⌜b = true⌝ ∗ ⌜can_commit h m h'⌝ ∗
-                      GHist ((sa, m) :: h') ∗ LHist rpc sa ((sa, m) :: hl)) ∨
-        (⌜b = false⌝ ∗ GHist h' ∗ LHist rpc sa hl) >>>.
+                      GHist ((sa, m) :: h') ∗ LHist cstate sa ((sa, m) :: hl) ∗ Q h m) ∨
+        (⌜b = false⌝ ∗ ⌜¬ can_commit h m h'⌝ ∗ GHist h' ∗ LHist cstate sa hl) >>>.
 
   Definition init_client_proxy_spec : Prop :=
     ∀ (sa : socket_address),
@@ -88,16 +89,16 @@ Definition run_spec : Prop :=
         KVS_address ⤇ KVS_si ∗
         sa ⤳ (∅, ∅) ∗
         free_ports (ip_of_address sa) {[port_of_address sa]} }}}
-      init_client_proxy (s_serializer KVS_serialization)
+      SI_init_client_proxy (s_serializer KVS_serialization)
                   #sa #KVS_address @[ip_of_address sa]
-    {{{ rpc, RET rpc; CanStart sa rpc }}}.
+    {{{ cstate, RET cstate; CanStart sa cstate }}}.
 
 Definition init_kvs_spec : Prop :=
   {{{ KVS_address ⤇ KVS_si ∗
         KVS_address ⤳ (∅,∅) ∗
         free_ports (ip_of_address KVS_address)
                    {[port_of_address KVS_address]} }}}
-      init_server (s_serializer KVS_serialization)
+      SI_init_server (s_serializer KVS_serialization)
         #KVS_address
         @[(ip_of_address KVS_address)]
     {{{ RET #(); True }}}.
@@ -120,7 +121,7 @@ Proof. econstructor; solve_inG. Qed.
 Section SI_Module.
   Context `{!anerisG Mdl Σ}.
 
-  Class SI_init `{!User_params} := {
+  Class SI_init `{!User_params, !KVS_snapshot_isolation_api} := {
      SI_init_module E :
         True ⊢ |={E}=> ∃ (SIRes : SI_resources Mdl Σ),
        GlobalInv ∗
@@ -138,22 +139,22 @@ End SI_Module.
 (* TODO: REMOVE THIS LATER, it's just an example of usage. *)
 Section Prove_of_t_body_of_some_example.
   Context `{!anerisG Mdl Σ}.
-  Context `{!User_params, !SI_resources Mdl Σ}.
-  Context (wr_spec : read_spec).
+  Context `{!User_params, !KVS_snapshot_isolation_api, !SI_resources Mdl Σ}.
+  Context (rd_spec : read_spec).
 
   Definition code_snippet : val :=
-    λ: "rpc" "k", read "rpc" "k".
+    λ: "cstate" "k", SI_read "cstate" "k".
 
-  Lemma code_snippet_proof sa (rpc : val) h m (k : Key) :
+  Lemma code_snippet_proof sa (cstate : val) h m (k : Key) :
      {{{ ⌜k ∈ KVS_keys⌝ ∗
-           TState rpc h (<[k:=#42]> m)}}}
-       code_snippet rpc #k @[ip_of_address sa]
+           TState cstate h (<[k:=#42]> m)}}}
+       code_snippet cstate #k @[ip_of_address sa]
      {{{ vo, RET vo; ⌜vo = $(Some 42)⌝ }}}.
  Proof.
    rewrite /code_snippet.
    iIntros (Φ) "(Hkey & HTState) HΦ".
    wp_pures.
-   iApply (wr_spec with "[$][$HTState]").
+   iApply (rd_spec with "[$][$HTState]").
    iNext.
    iIntros (vo) "(_ & [%Habs | %Hpost])"; iApply "HΦ";
      first by set_solver.
