aneris/examples/snapshot_isolation/snapshot_isolation_code_api.v
@@ -1,0 +1,28 @@
+
+From aneris.aneris_lang Require Import ast.
+From aneris.examples.snapshot_isolation
+     Require Import snapshot_isolation_code.
+
+
+Class KVS_snapshot_isolation_api :=
+  { SI_init_server : serializer -> val;
+    SI_start : val;
+    SI_read : val;
+    SI_write : val;
+    SI_commit : val;
+    SI_run : val;
+    SI_init_client_proxy : serializer -> val
+ }.
+
+(* TODO: move to the instantiation folder when ready. *)
+(*
+Global Instance KVS_snapshot_isolation_api_implementation : KVS_snapshot_isolation_api :=
+  {| SI_init_server := init_server;
+    SI_start := start;
+    SI_read := read;
+    SI_write := write;
+    SI_commit := commit;
+    SI_run := run;
+    SI_init_client_proxy := init_client_proxy;
+ |}.
+*)
